\documentclass[a4paper]{article}

\title{Transform relative effect vector to different baseline}

\begin{document}

\maketitle

Say we have a vector of relative effects $d$ against baseline $x$: $X = (d(x, w_1), d(x, w_2), \dots)^T$, and $X$ is normally distributed:
$$
X \sim \mathcal{N}(\mu, \Sigma)
$$

We want to change the baseline to $y$: $Y = (d(y, z_1), d(y, z_2), \dots)^T$, and derive a normal distribution like:
$$
Y \sim \mathcal{N}(\mu', \Sigma')
$$

Then, if we derive a matrix $B$ such that $Y = BX$, we have $\mu' = B\mu$ and $\Sigma' = B\Sigma B^T$. We can define $B$ as:
$$
B_{i,j} = \left\{
\begin{array}{ll}
-1 & \mathrm{if}\; w_j = y \\
1 & \mathrm{if}\; w_i = z_j \\
0 & \mathrm{otherwise}\\
\end{array}
\right.
$$

\end{document}
